Auto/Lib/IntExtra.lean
@@ -26,10 +26,6 @@ instance : LawfulBEq Int where
   eq_of_beq := Int.eq_of_beq_eq_true
   rfl := Int.beq_refl
 
-def Int.ge (a b : Int) := Int.le b a
-
-def Int.gt (a b : Int) := Int.lt b a
-
 def Int.abs (x : Int) := ite (x ≤ (-x)) (-x) x
 
 end Auto
