Auto/Lib/StringExtra.lean
@@ -2,10 +2,6 @@ namespace Auto
 
 @[reducible] def String.le (a b : String) : Prop := a = b ∨ a < b
 
-@[reducible] def String.ge (a b : String) : Prop := a = b ∨ b < a
-
 def String.lt (a b : String) : Prop := a < b
-
-def String.gt (a b : String) : Prop := b < a
 
 end Auto
