Auto/Translation/Lam2TH0.lean
@@ -7,7 +7,8 @@ open Lean Embedding.Lam Lam2TH0
 def lam2TH0 (lamVarTy : Array LamSort) (lamEVarTy : Array LamSort) (facts : Array LamTerm) : CoreM String := do
   let (typeHs, termHs, etomHs) ← LamReif.collectLamTermsAtoms lamVarTy lamEVarTy facts
   let bvHs := LamReif.collectLamTermsBitvecs facts
-  let bvLengthHs := HashSet.empty.insertMany (bvHs.toList.map List.length)
+  let bvLengthHs := LamReif.collectLamSortsBitVecLengths (
+    bvHs.toArray.map BitVecConst.lamCheck ++ lamVarTy ++ lamEVarTy)
   let ncHs := LamReif.collectLamTermsNatConsts facts
   let icHs := LamReif.collectLamTermsIntConsts facts
   let scHs := LamReif.collectLamTermsStringConsts facts
@@ -22,7 +23,7 @@ def lam2TH0 (lamVarTy : Array LamSort) (lamEVarTy : Array LamSort) (facts : Arra
     ncHs.toList.map (fun nc => s!"thf(typedecl_icst_{transNatConst nc}, type, {transNatConst nc}: {transNatConstSort nc}).") ++
     icHs.toList.map (fun ic => s!"thf(typedecl_icst_{transIntConst ic}, type, {transIntConst ic}: {transIntConstSort ic}).") ++
     scHs.toList.map (fun sc => s!"thf(typedecl_icst_{transStringConst sc}, type, {transStringConst sc}: {transStringConstSort sc}).") ++
-    bvHs.toList.map (fun l => s!"thf(typedecl_bv{transBitvec l}, type, t_bv{transBitvec l}: s_bv{l.length}).") ++
+    bvHs.toList.map (fun bvc => s!"thf(typedecl_bv{transBitVecConst bvc}, type, t_bv{transBitVecConst bvc}: {transBitVecConstSort bvc}).") ++
     (← termHs.toList.mapM (fun i => do
       let .some s := lamVarTy.get? i
         | throwError "lam2TH0 :: Unexpected error"
